src/SDK/Keyring/Defs.dfy
@@ -12,14 +12,22 @@ module KeyringDefs {
     method OnEncrypt(encMat: Materials.EncryptionMaterials) returns (res: Result<Materials.EncryptionMaterials>)
       requires Valid()
       requires encMat.Valid()
-      modifies encMat`plaintextDataKey, encMat`encryptedDataKeys
+      modifies encMat`plaintextDataKey, encMat`encryptedDataKeys, encMat`keyringTrace
       ensures Valid()
       ensures res.Success? ==> res.value.Valid() && res.value == encMat
       ensures res.Success? && old(encMat.plaintextDataKey.Some?) ==> res.value.plaintextDataKey == old(encMat.plaintextDataKey)
       ensures res.Failure? ==> unchanged(encMat)
-      // TODO: keyring trace GENERATED_DATA_KEY flag assurance
-      // TODO: keyring trace ENCRYPTED_DATA_KEY flag assurance
-
+      // if set plaintext data key on encrypt, keyring trace contains a new trace with the GENERATED_DATA_KEY flag.
+      ensures old(encMat.plaintextDataKey).None? && encMat.plaintextDataKey.Some? ==> (
+        |encMat.keyringTrace| > |old(encMat.keyringTrace)| &&
+        exists trace :: trace in encMat.keyringTrace[|old(encMat.keyringTrace)|..] && Materials.GENERATED_DATA_KEY in trace.flags
+      )
+      // if added a new encryptedDataKey, keyring trace contains a new trace with the ENCRYPTED_DATA_KEY flag.
+      ensures |encMat.encryptedDataKeys| > |old(encMat.encryptedDataKeys)| ==> (
+        |encMat.keyringTrace| > |old(encMat.keyringTrace)| &&
+        exists trace :: trace in encMat.keyringTrace[|old(encMat.keyringTrace)|..] && Materials.ENCRYPTED_DATA_KEY in trace.flags
+      )
+        
     method OnDecrypt(decMat: Materials.DecryptionMaterials, edks: seq<Materials.EncryptedDataKey>) returns (res: Result<Materials.DecryptionMaterials>)
       requires Valid()
       requires decMat.Valid()
@@ -30,6 +38,11 @@ module KeyringDefs {
       ensures old(decMat.plaintextDataKey.Some?) ==> res.Success? && unchanged(decMat)
       ensures res.Success? ==> res.value == decMat
       ensures res.Failure? ==> unchanged(decMat)
-      // TODO: keyring trace DECRYPTED_DATA_KEY flag assurance
+      // if set plaintext data key on decrypt, keyring trace contains a new trace with the DECRYPTED_DATA_KEY flag.
+      ensures old(decMat.plaintextDataKey).None? && decMat.plaintextDataKey.Some? ==> (
+        |decMat.keyringTrace| > |old(decMat.keyringTrace)| &&
+        |decMat.keyringTrace[|old(decMat.keyringTrace)|..]| > 0 &&
+        exists trace :: trace in decMat.keyringTrace[|old(decMat.keyringTrace)|..] && Materials.DECRYPTED_DATA_KEY in trace.flags
+      )
   }
 }
